src/examples/matmul/GPU.MatMul.Impure.fsti
@@ -6,6 +6,7 @@ open FStar.Mul
 open Pulse.Lib.Pervasives
 open Pulse.Lib.BigStar
 open GPU
+module U64 = FStar.UInt64
 
 module SZ = FStar.SizeT
 open FStar.SizeT
@@ -39,6 +40,8 @@ val gpu_matrix_unshare_underspec
     (bigstar #uid 0 shared (fun _ -> gpu_pts_to_matrix #a rows columns ga shared s))
     (fun _ -> gpu_pts_to_matrix #a rows columns ga 1 s)
 
+[@@CPrologue "__device__"]
+inline_for_extraction
 ```pulse
 fn gpu_matrix_read
   #a
@@ -65,4 +68,36 @@ fn gpu_matrix_read
   v
 }
 ```
+
+// fixme, function above extracts wrongly (returns void* instead of uint64_t in
+// the specialization). If the inline_for_extraction was not there above, the
+// resulting C code would not typecheck.
+[@@CPrologue "__device__"]
+inline_for_extraction
+```pulse
+fn gpu_matrix_read_u64
+  (#rows #columns: SZ.t)
+  (ga : gpu_array U64.t (rows * columns))
+  (#shared: erased nat{shared > 0})
+  (#s: erased (Seq.Base.seq U64.t) { Seq.length s == rows * columns })
+  (row: SZ.t{SZ.v row < rows})
+  (col: SZ.t{SZ.v col < columns})
+  requires gpu ** gpu_pts_to_matrix rows columns ga shared s
+  returns v: U64.t
+  // TODO: is the assert here opaque?
+  ensures gpu ** gpu_pts_to_matrix rows columns ga shared s ** pure (assert ((SZ.v row + 1) * columns <= rows * columns); v == Seq.Base.index s (row * columns + SZ.v col))
+{
+  assume_ (pure (forall (x:nat). SizeT.fits x)); // CHEATING overflow
+  unfold gpu_pts_to_matrix rows columns ga shared s;
+  unfold gpu_pts_to_array ga #(Real.one /. Real.of_int shared) s;
+  // TODO: strange that commenting this out causes an error
+  assert (pure ((row + 1) * columns <= rows * columns));
+  let idx = row *^ columns +^ col;
+  let v = gpu_array_read #U64.t #(rows * columns) #0 #(rows * columns) ga #(Real.one /. Real.of_int shared) idx #s;
+  fold gpu_pts_to_array ga #(Real.one /. Real.of_int shared) s;
+  fold gpu_pts_to_matrix rows columns ga shared s;
+  v
+}
+```
+
 #pop-options
